First draft of the valid_bplustree Prop.

code/bpt_proofs.v
@@ -85,4 +85,110 @@ Proof.
       apply list_tail_is_sorted in H. apply H.
 Qed.    
     
+
+
+
+(* Some props for having a prop apply to all elements in a list *)
+Inductive all_values (X : Type) (P : X -> Prop) : list (nat * X) -> Prop :=
+  | av_empty : all_values X P []
+  | av_next : forall (x:X) (n: nat) (l: list (nat * X)), all_values X P l -> P x -> all_values X P ((n,x)::l)
+.
+Inductive all_keys (X : Type) (P : nat -> Prop) : list (nat * X) -> Prop :=
+  | ak_empty : all_keys X P []
+  | ak_next : forall (x:X) (n: nat) (l: list (nat * X)), all_keys X P l -> P n -> all_keys X P ((n,x)::l)
+.
+
+(* Some helper functions for checking if a number is above or below a given number *)
+Definition below (n: nat) : nat -> Prop :=
+  fun o => blt_nat o n = true. 
+Definition between (n m: nat) : nat -> Prop :=
+  fun o => andb (ble_nat n o) (blt_nat o m) = true.
+Definition above (m: nat) : nat -> Prop :=
+  fun o => ble_nat m o = true.
+
+(* Prop for determining if the splitting points indicated actually are splits *)
+Inductive valid_splits' (b: nat) (X: Type) : list (nat * bplustree b X) -> Prop :=
+  | valid_p : forall (t1 t2: bplustree b X) (n1 n2: nat) (l: list (nat * bplustree b X)),
+              all_keys X (between n1 n2) (all_members t1) ->
+              valid_splits' b X ((n2, t2)::l) ->
+              valid_splits' b X ((n1, t1)::(n2, t2)::l)
+  | valid_ep : forall (t: bplustree b X) (n: nat),
+               all_keys X (above n) (all_members t) ->
+               valid_splits' b X ((n, t)::[]).
+Inductive valid_splits (b: nat) (X: Type) : bplustree b X -> list (nat * bplustree b X) -> Prop :=
+  | valid_sp : forall (t1 t2: bplustree b X) (n: nat) (l: list (nat * bplustree b X)),
+               all_keys X (below n) (all_members t1) ->
+               valid_splits' b X ((n, t2)::l) -> 
+               valid_splits b X t1 ((n, t2)::l).
+
+(* Prop for determining if a subtree is a valid subtree *)
+Inductive valid_sub_bplustree (b: nat) (X: Type) : bplustree b X -> Prop :=
+  | valid_leaf : forall (l: list (nat * X)), 
+                     b <= length(l) -> 
+                     length(l) <= mult b 2 ->
+                     kvl_sorted l ->  
+                     valid_sub_bplustree b X (bptLeaf b X l)
+  | valid_node : forall (sp: bplustree b X) (kpl: list (nat * bplustree b X)), 
+                      b <= length(kpl) -> 
+                      length(kpl) <= mult b 2 -> 
+                      valid_sub_bplustree b X sp ->
+                      all_values (bplustree b X) (valid_sub_bplustree b X) kpl ->
+                      kvl_sorted kpl ->
+                      valid_splits b X sp kpl -> 
+                      valid_sub_bplustree b X (bptNode b X sp kpl)   
+.
+
+(* Main prop that determines if an entire B+-tree is valid *)
+Inductive valid_bplustree (b: nat) (X: Type) : bplustree b X -> Prop :=
+  | root_is_a_leaf : forall (l: list (nat * X)), 
+                     length(l) <= mult b 2 ->
+                     kvl_sorted l ->  
+                     valid_bplustree b X (bptLeaf b X l)
+  | valid_root_node : forall (sp: bplustree b X) (kpl: list (nat * bplustree b X)), 
+                      length(kpl) <> 0 -> 
+                      length(kpl) <= mult b 2 -> 
+                      valid_sub_bplustree b X sp ->
+                      all_values (bplustree b X) (valid_sub_bplustree b X) kpl ->
+                      kvl_sorted kpl -> 
+                      valid_splits b X sp kpl -> 
+                      valid_bplustree b X (bptNode b X sp kpl)   
+.
+
+(* Some smaller examples *)
+Example valid_empty_tree : valid_bplustree 1 nat (bptLeaf 1 nat []).
+Proof. apply root_is_a_leaf. simpl. omega. apply kvl_sorted_0. Qed.
+Example valid_tiny_tree : valid_bplustree 1 nat (bptLeaf 1 nat [(1, 11), (2,22)]).
+Proof.  apply root_is_a_leaf. simpl. omega. apply kvl_sorted_cons. apply kvl_sorted_1. reflexivity. Qed.
+Example invalid_bigger_tree : ~ (valid_bplustree 1 nat (bptLeaf 1 nat [(1, 11), (2,22), (3, 33)])).
+Proof. unfold not. intro. inversion H. simpl in H1. inversion H1. inversion H4. inversion H6. Qed.
+
+(* 3 Examples all showing the same - that our demo `root` B+-tree is valid *)
+Example valid_small_tree : valid_bplustree 1 nat root.
+Proof. compute. apply valid_root_node. 
+  Case "has enough items". simpl. omega.
+  Case "doesnt have too many items". simpl. omega. 
+  Case "sp". apply valid_leaf.  simpl.  omega. simpl. omega. apply kvl_sorted_1.
+  Case "kvl". apply av_next. apply av_next. apply av_empty.
+    apply valid_leaf. simpl. omega.  simpl. omega. apply kvl_sorted_1.
+    apply valid_leaf. simpl. omega.  simpl. omega. apply kvl_sorted_1.
+  Case "valid sorting". 
+    apply kvl_sorted_cons. apply kvl_sorted_1. reflexivity.
+  Case "valid splits". 
+  apply valid_sp. apply ak_next. apply ak_empty. reflexivity.
+  apply valid_p. apply ak_next. apply ak_empty. reflexivity.
+  apply valid_ep. apply ak_next. apply ak_empty. reflexivity.
+Qed.
+Example valid_small_tree' : valid_bplustree 1 nat root.
+Proof. compute.
+  constructor. 
+  Case "has enough items". simpl. omega.
+  Case "doesnt have too many items". simpl. omega. 
+  Case "sp". repeat constructor. 
+  Case "kvl". repeat constructor.
+  Case "valid sorting". repeat constructor.
+  Case "valid splits". repeat constructor.
+Qed.
+Example valid_small_tree'' : valid_bplustree 1 nat root.
+Proof. compute. repeat constructor. simpl. omega. Qed.
+
     
